trait feasability

src/MutableMap/MutableMapFeasability-java/MutableMap/MutableMap.java
@@ -1,0 +1,63 @@
+/*******************************************************************************
+*  Copyright by the contributors to the Dafny Project
+*  SPDX-License-Identifier: MIT
+*******************************************************************************/
+package MutableMap;
+
+import dafny.DafnySet;
+import dafny.DafnyMap;
+import dafny.Tuple2;
+import dafny.TypeDescriptor;
+
+import java.util.HashMap;
+import java.util.ArrayList;
+import java.util.Map;
+
+
+public class MutableMap<K,V> {
+  private HashMap<K, V> m;
+
+  public DafnyMap<K,V> content() {
+    return new DafnyMap<>(m);
+  }
+
+  public MutableMap() {
+    m = new HashMap<>();
+  }
+
+  public MutableMap(TypeDescriptor<K> x, TypeDescriptor<V> y) {
+    m = new HashMap<>();
+  }
+
+  public void put(K k, V v) {
+    m.put(k, v);
+  }
+
+  public DafnySet<? extends K> keys() {
+    return new DafnySet<>(m.keySet());
+  }
+
+  public DafnySet<? extends V> values() {
+    return new DafnySet<>(m.values());
+  }
+
+  public DafnySet<? extends Tuple2<K,V>> items() {
+    ArrayList<Tuple2<K, V>> list = new ArrayList<Tuple2<K, V>>();
+    for (Map.Entry<K, V> entry : m.entrySet()) {
+      list.add(new Tuple2<K, V>(entry.getKey(), entry.getValue()));
+    }
+    return new DafnySet<Tuple2<K, V>>(list);
+  }
+
+  public V find(K k) {
+    return m.get(k);
+  }
+
+  public void remove(K k) {
+    m.remove(k);
+  }
+
+  public int size() {
+    return m.size();
+  }
+}
