src/MutableMap/MutableMapFeasability.dfy
@@ -1,10 +1,57 @@
 include "MutableMap.dfy"
 
-module {:options "/functionSyntax:4"} MutableMapFeasability refines MutableMap {
-  class MutableMap<K(==),V(==)> ... {
+/*******************************************************************************
+*  Copyright by the contributors to the Dafny Project
+*  SPDX-License-Identifier: MIT
+*******************************************************************************/
+
+// RUN: %dafny /compile:0 "%s"
+
+module {:options "/functionSyntax:4"} MutableMapTrait {
+  trait MutableMapTrait<K(==),V(==)> {
+    function content(): map<K, V>
+      reads this
+
+    method Put(k: K, v: V)
+      modifies this
+      ensures this.content() == old(this.content())[k := v]    
+
+    function Keys(): (keys: set<K>)
+      reads this
+      ensures keys == this.content().Keys
+
+    function Values(): (values: set<V>)
+      reads this
+      ensures values == this.content().Values
+
+    function Items(): (items: set<(K,V)>)
+      reads this
+      ensures items == this.content().Items
+      ensures items == set k | k in this.content().Keys :: (k, this.content()[k])
+
+    function Find(k: K): (v: V)
+      reads this
+      requires k in this.Keys()
+      ensures v in this.content().Values
+      ensures this.content()[k] == v
+    
+    method Remove(k: K)
+      modifies this
+      ensures this.content() == old(this.content()) - {k}
+
+    function Size(): (size: int)
+      reads this
+      ensures size == |this.content().Items|
+  }
+}
+
+module {:options "/functionSyntax:4"} MutableMapFeasability refines MutableMapTrait {
+  class MutableMap<K(==),V(==)> extends MutableMapTrait<K,V> {
     var m: map<K,V>
 
-    function content(): map<K, V> {
+    function content(): map<K, V> 
+      reads this
+    {
       m
     }
 
@@ -14,21 +61,30 @@ module {:options "/functionSyntax:4"} MutableMapFeasability refines MutableMap {
     }
 
     method Put(k: K, v: V) 
+      modifies this
+      ensures this.content() == old(this.content())[k := v] 
     {
       m := m[k := v];
     }
 
-    function Keys(): set<K>
+    function Keys(): (keys: set<K>)
+      reads this
+      ensures keys == this.content().Keys
     {
       m.Keys
     }
 
-    function Values(): set<V>
+    function Values(): (values: set<V>)
+      reads this
+      ensures values == this.content().Values
     {
       m.Values
     }
 
-    function Items(): set<(K,V)>
+    function Items(): (items: set<(K,V)>)
+      reads this
+      ensures items == this.content().Items
+      ensures items == set k | k in this.content().Keys :: (k, this.content()[k])
     {
       var items := set k | k in m.Keys :: (k, m[k]);
       assert items == m.Items by {
@@ -45,16 +101,24 @@ module {:options "/functionSyntax:4"} MutableMapFeasability refines MutableMap {
     }
 
     function Find(k: K): (v: V)
+      reads this
+      requires k in this.Keys()
+      ensures v in this.content().Values
+      ensures this.content()[k] == v
     {
       m[k]
     }
 
     method Remove(k: K)
+      modifies this
+      ensures this.content() == old(this.content()) - {k}
     {
       m := map k' | k' in m.Keys && k' != k :: m[k'];
     }
 
     function Size(): (size: int)
+      reads this
+      ensures size == |this.content().Items|
     {
       |m|
     }
